backend/Tailcallproof.v
@@ -309,6 +309,15 @@ Proof.
   eapply (Genv.match_genvs_allowed_calls TRANSL). eauto.
 Qed.
 
+Lemma allowed_syscall_translated:
+  forall cp ef,
+    Genv.allowed_syscall ge cp ef ->
+    Genv.allowed_syscall tge cp ef.
+Proof.
+  intros cp ef H.
+  eapply (Genv.match_genvs_allowed_syscalls TRANSL). eauto.
+Qed.
+
 Lemma find_comp_translated:
   forall vf,
     Genv.find_comp_in_genv ge vf = Genv.find_comp_in_genv tge vf.
@@ -743,6 +752,7 @@ Proof.
   eapply eval_builtin_args_preserved with (ge1 := ge); eauto. exact symbols_preserved.
   eapply external_call_symbols_preserved; eauto. apply senv_preserved.
   rewrite comp_transf_function; eauto.
+  rewrite comp_transf_function; eauto using allowed_syscall_translated.
   econstructor; eauto.
   (* TODO: Should be a lemma! *)
   { clear -A STACKS.
@@ -826,6 +836,7 @@ Proof.
   left. exists (Returnstate s' res' m2' bottom); split.
   simpl. econstructor; eauto.
   eapply external_call_symbols_preserved; eauto. apply senv_preserved.
+  eauto using allowed_syscall_translated.
   constructor; auto.
   (* TODO: Should be a lemma? *)
   { clear -A H6.
